theories/examples/even.v
@@ -1,0 +1,200 @@
+From iris.program_logic Require Import lifting adequacy.
+From RobustSafety Require Import lang rules logrel fundamental.
+From iris.proofmode Require Import tactics.
+
+(* The program 'prog' below corresponfs to the following program:
+
+let l = ref(0) in
+let add2 () = FAA(l, 2); () in
+let read () =
+  let r = !l in
+  assert (r `rem` 2 = 0); r
+in
+(add2, read)
+*)
+Definition even_reference : expr :=
+  LetIn
+    (Alloc (#n 0))
+    (Pair
+       (Lam (Seq (FAA (Var 1) (#n 2)) Unit))
+       (Lam (LetIn
+               (Load (Var 1))
+               (Seq (Assert (BinOp Eq (BinOp Rem (Var 0) (#n 2)) (#n 0))) (Var 0))))).
+
+(* is this a Coq bug!? why is modulo unfolded by simpl? *)
+Opaque Nat.modulo.
+
+Section even.
+  Context `{heapIG Σ}.
+
+  Definition add2_spec (add2 : val) : iProp Σ :=
+    ∀ v, {{{ True }}} App (of_val add2) (of_val v) {{{ RET UnitV; True }}}.
+
+  Definition read_spec (read : val) : iProp Σ :=
+    ∀ v, {{{ True }}} App (of_val read) (of_val v) {{{ n, RET (#nv n); ⌜(2 | n)⌝ }}}.
+
+  Lemma wp_even_reference :
+    {{{ True }}}
+      even_reference
+    {{{ add2 read, RET (PairV add2 read);
+        interp add2 ∗ interp read ∗ add2_spec add2 ∗ read_spec read }}}.
+  Proof.
+    iIntros (Φ) "_ HΦ".
+    iApply (wp_bind (fill [LetInCtx _])).
+    iApply wp_alloc; first done.
+    iNext.
+    iIntros (l) "Hl /=".
+    iMod (inv_alloc (nroot .@ "even") _ (∃ n, l ↦ (#nv n) ∧ ⌜(2 | n)⌝)%I with "[Hl]") as "#Hinv".
+    { iNext; iExists _; iFrame. iPureIntro. apply Nat.divide_0_r. }
+    iApply wp_pure_step_later; first done.
+    iNext; iIntros "_".
+    asimpl.
+    iApply wp_value.
+    iApply "HΦ".
+    set (add2V := LamV (Seq (FAA (Loc l) (#n 2)) Unit)).
+    set (readV := (LamV (LetIn (Load (Loc l))
+          (Seq (Assert (BinOp Eq (BinOp Rem (ids 0) (#n 2)) (#n 0))) (ids 0))))).
+    iAssert (add2_spec add2V ∗ read_spec readV)%I as "#[Has Hrs]".
+    { iSplit.
+      - iIntros (v Ψ) "!# _ HΨ /=".
+        iApply wp_pure_step_later; first done.
+        iNext; iIntros "_".
+        simpl.
+        iApply (wp_bind (fill [SeqCtx _])).
+        iInv (nroot .@ "even") as (n) ">[Hl %]" "Hclose".
+        iApply (wp_FAA with "Hl").
+        iIntros "!> Hl".
+        iMod ("Hclose" with "[Hl]") as "_".
+        { iNext; iExists _; iFrame. iPureIntro.
+          apply Nat.divide_add_r; first done. apply Nat.divide_refl. }
+        simpl.
+        iModIntro.
+        iApply wp_pure_step_later; first done.
+        iNext; iIntros "_".
+        iApply wp_value.
+        by iApply "HΨ".
+      - iIntros (v Ψ) "!# _ HΨ /=".
+        iApply wp_pure_step_later; first done.
+        iNext; iIntros "_".
+        asimpl.
+        iApply (wp_bind (fill [LetInCtx _])).
+        asimpl.
+        iInv (nroot .@ "even") as (n) ">[Hl %]" "Hclose".
+        iApply (wp_load with "Hl").
+        iIntros "!> Hl".
+        iMod ("Hclose" with "[Hl]") as "_".
+        { iNext; iExists _; iFrame; done. }
+        simpl.
+        iModIntro.
+        iApply wp_pure_step_later; first done.
+        iNext; iIntros "_".
+        asimpl.
+        iApply (wp_bind (fill [SeqCtx _])).
+        iApply (wp_bind (fill [AssertCtx])).
+        iApply (wp_bind (fill [BinOpLCtx _ _])).
+        iApply wp_pure_step_later; first done.
+        iNext; iIntros "_".
+        iApply wp_value; simpl.
+        iApply wp_pure_step_later; first done.
+        iNext; iIntros "_".
+        simpl.
+        rewrite bool_decide_eq_true_2; last by rewrite Nat.mod_divide.
+        iApply wp_value; simpl.
+        iApply wp_pure_step_later; first done.
+        iNext; iIntros "_".
+        iApply wp_value; simpl.
+        iApply wp_pure_step_later; first done.
+        iNext; iIntros "_".
+        iApply wp_value.
+        iApply "HΨ"; done. }
+    repeat iSplit; [| |done|done].
+    - rewrite interp_unfold /=.
+      iIntros "!#" (v) "_".
+      iApply wp_stuck_weaken.
+      iApply ("Has" $! v with "[] []"); [done|rewrite interp_unfold //=].
+    - rewrite interp_unfold /=.
+      iIntros "!#" (v) "_".
+      iApply wp_stuck_weaken.
+      iApply ("Hrs" $! v with "[] []"); [done|].
+      iNext; iIntros (? ?); rewrite interp_unfold //=.
+  Qed.
+
+  Definition even_linked_with_adversary (e : expr) : expr :=
+    LetIn
+      even_reference
+      (LetIn (Fst (Var 0))
+         (LetIn (Snd (Var 1))
+            (Seq e (App (Var 0) Unit)))).
+
+  Lemma even_linked_with_adversary_spec e :
+    valid_adversary e →
+    {{{ True }}} even_linked_with_adversary e ? {{{ n, RET (#nv n); ⌜(2 | n)⌝ }}}.
+  Proof.
+    iIntros (Hvad Φ) "_ HΦ".
+    iApply (wp_bind (fill [LetInCtx _])).
+    iApply wp_stuck_weaken.
+    iApply wp_even_reference; first done.
+    iNext.
+    iIntros (add2 read) "(#Hai & #Hri & #Has & #Hrs) /=".
+    iApply wp_pure_step_later; first done.
+    iNext; iIntros "_". asimpl.
+    iApply (wp_bind (fill [LetInCtx _])).
+    iApply wp_pure_step_later; first done.
+    iNext; iIntros "_".
+    iApply wp_value.
+    asimpl.
+    iApply wp_pure_step_later; first done.
+    iNext; iIntros "_".
+    asimpl.
+    iApply (wp_bind (fill [LetInCtx _])).
+    iApply wp_pure_step_later; first done.
+    iNext; iIntros "_".
+    iApply wp_value.
+    asimpl.
+    iApply wp_pure_step_later; first done.
+    iNext; iIntros "_".
+    asimpl.
+    iApply (wp_bind (fill [SeqCtx _])).
+    iApply wp_wand.
+    { iApply (fundamental _ Hvad $! [read; add2; PairV add2 read] with "[]").
+      rewrite !interp_env_cons.
+      repeat iSplit; [done|done|by rewrite {3}interp_unfold /=; eauto 10|by iApply interp_env_nil]. }
+    iIntros (v) "Hv /=".
+    iApply wp_pure_step_later; first done.
+    iNext; iIntros "_".
+    iApply wp_stuck_weaken.
+    iApply ("Hrs" $! UnitV); done.
+  Qed.
+
+End even.
+
+Theorem even_robust_safety :
+  ∀ e,
+    valid_adversary e →
+    ∀ n κs v t2 σ2,
+      language.nsteps n ([(even_linked_with_adversary e)], {|Heap := ∅; Failure := false|})
+        κs (of_val v :: t2, σ2) →
+      Failure σ2 = false ∧ ∃ n, v = #nv n.
+Proof.
+  intros e He n κs v t2 σ2.
+  eapply (wp_strong_adequacy heapΣ _).
+  iIntros (Hinv).
+  iMod (gen_heap_init (∅ : gmap loc val)) as (?) "(Hh&_&_)".
+  set (HeapIG heapΣ _ _).
+  iAssert (WP even_linked_with_adversary e ? {{v, ∃ n, ⌜v = (#nv n)⌝}})%I as "Hwp".
+  { iApply (even_linked_with_adversary_spec with "[] []"); [done|done|by eauto]. }
+  iModIntro.
+  iExists _, [_]%I, _, _; simpl.
+  iSplitL; last iSplitL; [|iSplitL; last done; iExact "Hwp" |].
+  { by simpl; iFrame. }
+  iIntros (es' t2' Hv Hes' _) "[Hh %] Hposts _ /=".
+  iMod (fupd_mask_weaken ∅ (P := True) with "[]") as "_"; first done.
+  { iIntros "?"; iModIntro; done. }
+  iModIntro.
+  destruct es' as [|ev []]; [done| |done]; simpl.
+  iDestruct "Hposts" as "[Hposts _]".
+  pose proof (f_equal head Hv); simpl in *; simplify_eq.
+  rewrite to_of_val /=.
+  iDestruct "Hposts" as (?) "->".
+  by eauto.
+Qed.
